more

Weidenbach_Book/IsaSAT_Propagate_Conflict.thy
@@ -41,40 +41,6 @@ prepare_code_thms (in -) watched_by_app_heur_code_def
 lemmas watched_by_app_heur_code_refine[sepref_fr_rules] =
    watched_by_app_heur_code.refine[of \<A>\<^sub>i\<^sub>n, OF isasat_input_bounded_axioms]
 
-(* TODO Kill *)
-lemma watched_by_app_code_refine[sepref_fr_rules]:
-  \<open>(uncurry2 watched_by_app_heur_code, uncurry2 (RETURN ooo watched_by_app)) \<in>
-    [\<lambda>((S, L), K).  L \<in> snd ` D\<^sub>0 \<and> K < length (watched_by S L)]\<^sub>a
-       twl_st_assn\<^sup>k *\<^sub>a unat_lit_assn\<^sup>k *\<^sub>a nat_assn\<^sup>k \<rightarrow>
-    nat_assn\<close>
-    (is \<open>_ \<in> [?pre]\<^sub>a ?im \<rightarrow> ?f\<close>)
-proof -
-  have H: \<open>(uncurry2 watched_by_app_heur_code, uncurry2 (RETURN \<circ>\<circ>\<circ> watched_by_app))
-  \<in> [comp_PRE (twl_st_heur \<times>\<^sub>f Id \<times>\<^sub>f nat_rel)
-      (\<lambda>((S, L), K). L \<in> snd ` D\<^sub>0 \<and> K < length (get_watched_wl S L))
-      (\<lambda>_ ((S, L), K).
-          nat_of_lit L < length (get_watched_wl_heur S) \<and>
-          K < length (watched_by_int S L)) (\<lambda>_. True)]\<^sub>a
-    hrp_comp (twl_st_heur_assn\<^sup>k *\<^sub>a unat_lit_assn\<^sup>k *\<^sub>a nat_assn\<^sup>k)
-             (twl_st_heur \<times>\<^sub>f Id \<times>\<^sub>f nat_rel) \<rightarrow>
-    hr_comp nat_assn nat_rel\<close>
-    (is \<open>_ \<in> [?pre']\<^sub>a ?im' \<rightarrow> ?f'\<close>)
-    using hfref_compI_PRE_aux[OF watched_by_app_heur_code_refine[unfolded PR_CONST_def]
-        watched_by_app_watched_by_app_heur[unfolded PR_CONST_def],
-        unfolded watched_by_app_heur_pre_def] .
-  have pre: \<open>?pre' = ?pre\<close>
-    by (intro ext) (auto simp: comp_PRE_def twl_st_assn_def twl_st_heur_def map_fun_rel_def)
-  have im: \<open>?im' = ?im\<close>
-    unfolding prod_hrp_comp hrp_comp_dest hrp_comp_keep twl_st_assn_def[symmetric]
-    by (auto simp: hrp_comp_def hr_comp_def)
-  have f: \<open>?f' = ?f\<close>
-    unfolding prod_hrp_comp hrp_comp_dest hrp_comp_keep
-    by (auto simp: hrp_comp_def hr_comp_def)
-  show ?thesis
-    using H unfolding im pre f .
-qed
-
-
 sepref_thm access_lit_in_clauses_heur_code
   is \<open>uncurry2 (RETURN ooo access_lit_in_clauses_heur)\<close>
   :: \<open>[access_lit_in_clauses_heur_pre]\<^sub>a
@@ -99,41 +65,6 @@ lemma access_lit_in_clauses_heur_access_lit_in_clauses:
    twl_st_heur \<times>\<^sub>f nat_rel \<times>\<^sub>f nat_rel \<rightarrow>\<^sub>f \<langle>Id\<rangle> nres_rel\<close>
   by (intro frefI nres_relI)
      (auto simp: access_lit_in_clauses_heur_def twl_st_heur_def access_lit_in_clauses_def)
-
-(* TODO Kill *)
-lemma access_lit_in_clauses_refine[sepref_fr_rules]:
-  \<open>(uncurry2 access_lit_in_clauses_heur_code, uncurry2 (RETURN ooo access_lit_in_clauses)) \<in>
-    [\<lambda>((S, i), j). i < length (get_clauses_wl S) \<and> j < length_rll (get_clauses_wl S) i]\<^sub>a
-       twl_st_assn\<^sup>k *\<^sub>a nat_assn\<^sup>k *\<^sub>a nat_assn\<^sup>k \<rightarrow>
-    unat_lit_assn\<close>
-    (is \<open>_ \<in> [?pre]\<^sub>a ?im \<rightarrow> ?f\<close>)
-proof -
-  have H: \<open>(uncurry2 access_lit_in_clauses_heur_code, uncurry2 (RETURN \<circ>\<circ>\<circ> access_lit_in_clauses))
-  \<in> [comp_PRE (twl_st_heur \<times>\<^sub>f nat_rel \<times>\<^sub>f nat_rel) (\<lambda>_. True)
-      (\<lambda>_ (((_, N, _), i), j). i < length N \<and> j < length_rll N i) (\<lambda>_. True)]\<^sub>a
-    hrp_comp (twl_st_heur_assn\<^sup>k *\<^sub>a nat_assn\<^sup>k *\<^sub>a nat_assn\<^sup>k)
-             (twl_st_heur \<times>\<^sub>f nat_rel \<times>\<^sub>f nat_rel) \<rightarrow>
-    hr_comp unat_lit_assn Id\<close>
-    (is \<open>_ \<in> [?pre']\<^sub>a ?im' \<rightarrow> ?f'\<close>)
-    using hfref_compI_PRE_aux[OF access_lit_in_clauses_heur_code_refine[unfolded PR_CONST_def]
-        access_lit_in_clauses_heur_access_lit_in_clauses[unfolded PR_CONST_def],
-        unfolded access_lit_in_clauses_heur_pre_def] .
-  have pre: \<open>?pre x \<Longrightarrow> ?pre' x\<close> for x
-    unfolding comp_PRE_def
-      by (auto simp: comp_PRE_def twl_st_assn_def twl_st_heur_def
-          map_fun_rel_def intro!: ext)
-  have im: \<open>?im' = ?im\<close>
-    unfolding prod_hrp_comp hrp_comp_dest hrp_comp_keep twl_st_assn_def[symmetric]
-    by (auto simp: hrp_comp_def hr_comp_def)
-  have f: \<open>?f' = ?f\<close>
-    unfolding prod_hrp_comp hrp_comp_dest hrp_comp_keep
-    by (auto simp: hrp_comp_def hr_comp_def)
-  show ?thesis
-    apply (rule hfref_weaken_pre[OF ])
-     defer
-    using H unfolding im f apply assumption
-    using pre ..
-qed
 
 end
 
@@ -171,72 +102,6 @@ lemmas find_unwatched_wl_st_heur_code_find_unwatched_wl_st_heur[sepref_fr_rules]
    find_unwatched_wl_st_heur_code.refine[of \<A>\<^sub>i\<^sub>n, OF isasat_input_bounded_nempty_axioms,
      unfolded PR_CONST_def]
 
-(* TODO Kill *)
-theorem find_unwatched_wl_st_heur_code_find_unwatched_wl_s[sepref_fr_rules]:
-  \<open>(uncurry find_unwatched_wl_st_heur_code, uncurry find_unwatched_wl_st)
-    \<in> [\<lambda>(S, i). \<exists>w L. unit_prop_body_wl_D_inv S w L \<and> i = watched_by_app S L w]\<^sub>a
-      twl_st_assn\<^sup>k *\<^sub>a nat_assn\<^sup>k \<rightarrow> option_assn nat_assn\<close>
-    (is \<open>_ \<in> [?pre]\<^sub>a ?im \<rightarrow> ?f\<close>)
-proof -
-  have H: \<open>(uncurry find_unwatched_wl_st_heur_code, uncurry find_unwatched_wl_st)
-    \<in> [comp_PRE (twl_st_heur \<times>\<^sub>f nat_rel)
-         (\<lambda>(S, i). i < length (get_clauses_wl S) \<and> 0 < i \<and> literals_are_\<L>\<^sub>i\<^sub>n S \<and>
-            2 \<le> length (get_clauses_wl S ! i))
-         (\<lambda>_ (S, i). i < length (get_clauses_wl_heur S) \<and> 0 < i \<and> literals_are_in_\<L>\<^sub>i\<^sub>n_heur S)
-         (\<lambda>_. True)]\<^sub>a
-       hrp_comp (twl_st_heur_assn\<^sup>k *\<^sub>a nat_assn\<^sup>k)
-                   (twl_st_heur \<times>\<^sub>f nat_rel) \<rightarrow>
-       hr_comp (option_assn nat_assn) Id\<close>
-    (is \<open>_ \<in> [?pre']\<^sub>a ?im' \<rightarrow> ?f'\<close>)
-    using hfref_compI_PRE_aux[OF
-        find_unwatched_wl_st_heur_code_find_unwatched_wl_st_heur[unfolded PR_CONST_def]
-        find_unwatched_wl_st_heur_find_unwatched_wl_s,
-         unfolded find_unwatched_wl_st_heur_pre_def] .
-  have pre: \<open>?pre' x\<close> if \<open>?pre x\<close> for x
-  proof -
-    have [simp]: \<open>mset `# mset (take ai (tl ah)) + ak + (mset `# mset (drop (Suc ai) ah) + al) =
-      mset `# mset (tl ah) + ak + al\<close> for ai ah ak al
-      apply (subst (6) append_take_drop_id[of ai, symmetric])
-      unfolding mset_append drop_Suc
-      by auto
-    have [intro]: \<open>literals_are_in_\<L>\<^sub>i\<^sub>n_heur T\<close> and
-       \<open>get_clauses_wl_heur T = get_clauses_wl S\<close> if
-       \<open>is_\<L>\<^sub>a\<^sub>l\<^sub>l (all_lits_of_mm (cdcl\<^sub>W_restart_mset.clauses
-           (state\<^sub>W_of (twl_st_of None (st_l_of_wl None S)))))\<close> and
-       \<open>(T, S) \<in> twl_st_heur\<close>
-      for S and T
-      using that apply (auto simp: twl_st_heur_def mset_take_mset_drop_mset
-          mset_take_mset_drop_mset' clauses_def literals_are_in_\<L>\<^sub>i\<^sub>n_heur_def)
-      apply (auto simp add: all_lits_of_mm_union literals_are_in_\<L>\<^sub>i\<^sub>n_mm_def is_\<L>\<^sub>a\<^sub>l\<^sub>l_def)
-      done
-    show ?thesis
-      unfolding comp_PRE_def
-      apply (intro ext impI conjI)
-      subgoal
-        using that by (auto dest: simp: unit_prop_body_wl_D_inv_def unit_prop_body_wl_inv_def
-            unit_propagation_inner_loop_body_l_inv_def watched_by_app_def)
-      subgoal
-        by (use that in \<open>auto simp: comp_PRE_def unit_prop_body_wl_D_inv_def
-            mset_take_mset_drop_mset clauses_def mset_take_mset_drop_mset' drop_Suc
-            unit_prop_body_wl_inv_def watched_by_app_def
-            unit_propagation_inner_loop_body_l_inv_def twl_st_heur_def
-          simp del: twl_st_of.simps st_l_of_wl.simps\<close>)
-      done
-  qed
-  have im: \<open>?im' = ?im\<close>
-    unfolding prod_hrp_comp hrp_comp_dest hrp_comp_keep twl_st_assn_def[symmetric]
-    by (auto simp: hrp_comp_def hr_comp_def)
-  have f: \<open>?f' = ?f\<close>
-    unfolding prod_hrp_comp hrp_comp_dest hrp_comp_keep
-    by (auto simp: hrp_comp_def hr_comp_def)
-  show ?thesis
-    apply (rule hfref_weaken_pre[OF ])
-     defer
-    using H unfolding im f PR_CONST_def apply assumption
-    using pre ..
-qed
-
-
 sepref_thm set_conflict_wl_heur_code
   is \<open>uncurry set_conflict_wl_heur\<close>
   :: \<open>[set_conflict_wl_heur_pre]\<^sub>a
@@ -254,41 +119,6 @@ prepare_code_thms (in -) set_conflict_wl_heur_code_def
 
 lemmas set_conflict_wl_heur_code[sepref_fr_rules] =
   set_conflict_wl_heur_code.refine[OF isasat_input_bounded_nempty_axioms]
-
-lemma set_conflict_wl_heur_code_set_conflict_wl'[sepref_fr_rules]:
-  \<open>(uncurry set_conflict_wl_heur_code, uncurry (RETURN oo set_conflict_wl')) \<in>
-    [\<lambda>(C, S). get_conflict_wl S = None \<and> C < length (get_clauses_wl S) \<and>
-      distinct (get_clauses_wl S ! C) \<and> literals_are_in_\<L>\<^sub>i\<^sub>n (mset (get_clauses_wl S ! C)) \<and>
-      \<not> tautology (mset (get_clauses_wl S ! C)) \<and>
-      literals_are_in_\<L>\<^sub>i\<^sub>n_trail (get_trail_wl S)]\<^sub>a nat_assn\<^sup>k *\<^sub>a twl_st_assn\<^sup>d \<rightarrow>
-    twl_st_assn\<close>
-    (is \<open>_ \<in> [?pre]\<^sub>a ?im \<rightarrow> ?f\<close>)
-proof -
-  have H: \<open>(uncurry set_conflict_wl_heur_code, uncurry (RETURN \<circ>\<circ> set_conflict_wl'))
-  \<in> [comp_PRE (nat_rel \<times>\<^sub>f twl_st_heur) (\<lambda>_. True)
-       (\<lambda>_. set_conflict_wl_heur_pre)
-       (\<lambda>_. True)]\<^sub>a hrp_comp
-                       (nat_assn\<^sup>k *\<^sub>a twl_st_heur_assn\<^sup>d)
-                       (nat_rel \<times>\<^sub>f
-                        twl_st_heur) \<rightarrow> hr_comp
-           twl_st_heur_assn twl_st_heur\<close>
-    (is \<open>_ \<in> [?pre']\<^sub>a ?im' \<rightarrow> ?f'\<close>)
-    using hfref_compI_PRE_aux[OF set_conflict_wl_heur_code set_conflict_wl_heur_set_conflict_wl']
-    .
-  have pre: \<open>?pre' x\<close> if \<open>?pre x\<close> for x
-    using that unfolding comp_PRE_def twl_st_heur_def set_conflict_wl_heur_pre_def by auto
-  have im: \<open>?im' = ?im\<close>
-    unfolding prod_hrp_comp hrp_comp_dest hrp_comp_keep twl_st_assn_def[symmetric]
-    by (auto simp: hrp_comp_def hr_comp_def)
-  have f: \<open>?f' = ?f\<close>
-    unfolding prod_hrp_comp hrp_comp_dest hrp_comp_keep twl_st_assn_def
-    by (auto simp: hrp_comp_def hr_comp_def)
-  show ?thesis
-    apply (rule hfref_weaken_pre[OF ])
-     defer
-    using H unfolding im f PR_CONST_def apply assumption
-    using pre ..
-qed
 
 sepref_thm update_clause_wl_code
   is \<open>uncurry5 update_clause_wl_heur\<close>
@@ -313,93 +143,6 @@ prepare_code_thms (in -) update_clause_wl_code_def
 lemmas update_clause_wl_code[sepref_fr_rules] =
   update_clause_wl_code.refine[OF isasat_input_bounded_nempty_axioms]
 
-(* TODO Kill *)
-lemma update_clause_wl_code_update_clause_wl[sepref_fr_rules]:
-  \<open>(uncurry5 update_clause_wl_code, uncurry5 update_clause_wl) \<in>
-    [\<lambda>(((((L, C), w), i), f), S).
-      unit_prop_body_wl_D_inv S w L \<and>
-      unit_prop_body_wl_D_find_unwatched_inv (Some f) C S \<and>
-      C = watched_by S L ! w \<and>
-      i = (if get_clauses_wl S ! C ! 0 = L then 0 else 1)]\<^sub>a
-     unat_lit_assn\<^sup>k *\<^sub>a nat_assn\<^sup>k *\<^sub>a nat_assn\<^sup>k *\<^sub>a nat_assn\<^sup>k *\<^sub>a nat_assn\<^sup>k *\<^sub>a twl_st_assn\<^sup>d \<rightarrow>
-       nat_assn *a twl_st_assn\<close>
-    (is \<open>_ \<in> [?pre]\<^sub>a ?im \<rightarrow> ?f\<close>)
-proof -
-  have H: \<open>(uncurry5 update_clause_wl_code, uncurry5 update_clause_wl) \<in>
-    [comp_PRE (Id \<times>\<^sub>f nat_rel \<times>\<^sub>f nat_rel \<times>\<^sub>f nat_rel \<times>\<^sub>f nat_rel \<times>\<^sub>f twl_st_heur)
-       (\<lambda>(((((L, C), w), i), f), S). get_clauses_wl S ! C ! f \<noteq> L)
-       (\<lambda>_ (((((L, C), w), i), f), S).
-           C < length (get_clauses_wl_heur S) \<and>
-           f < length (get_clauses_wl_heur S ! C) \<and>
-           i < length (get_clauses_wl_heur S ! C) \<and>
-           nat_of_lit L < length (get_watched_wl_heur S) \<and>
-           nat_of_lit (get_clauses_wl_heur S ! C ! f)
-           < length (get_watched_wl_heur S) \<and>
-           w < length (get_watched_wl_heur S ! nat_of_lit L)) (\<lambda>_. True)]\<^sub>a
-    hrp_comp (unat_lit_assn\<^sup>k *\<^sub>a nat_assn\<^sup>k *\<^sub>a nat_assn\<^sup>k *\<^sub>a nat_assn\<^sup>k *\<^sub>a nat_assn\<^sup>k *\<^sub>a
-        twl_st_heur_assn\<^sup>d)
-      (Id \<times>\<^sub>f nat_rel \<times>\<^sub>f nat_rel \<times>\<^sub>f nat_rel \<times>\<^sub>f nat_rel \<times>\<^sub>f twl_st_heur) \<rightarrow>
-    hr_comp (nat_assn *a twl_st_heur_assn) (nat_rel \<times>\<^sub>f twl_st_heur)\<close>
-    (is \<open>_ \<in> [?pre']\<^sub>a ?im' \<rightarrow> ?f'\<close>)
-    using hfref_compI_PRE_aux[OF update_clause_wl_code update_clause_wl_heur_update_clause_wl]
-    unfolding update_clause_wl_code_pre_def
-    .
-  have [dest]: \<open>literals_are_in_\<L>\<^sub>i\<^sub>n_mm (mset `# mset (tl (get_clauses_wl S)))\<close>
-    if \<open>unit_prop_body_wl_D_inv S w L\<close>
-    for S w L
-  proof -
-    have \<open>literals_are_\<L>\<^sub>i\<^sub>n S\<close>
-      using that unfolding twl_st_heur_def map_fun_rel_def
-        unit_prop_body_wl_D_find_unwatched_inv_def
-        unit_prop_body_wl_find_unwatched_inv_def unit_prop_body_wl_D_inv_def
-        unit_prop_body_wl_inv_def
-        unit_propagation_inner_loop_body_l_inv_def by fast
-    then have \<open> set_mset (all_lits_of_mm (mset `# mset (tl (get_clauses_wl S)))) \<subseteq>
-       set_mset \<L>\<^sub>a\<^sub>l\<^sub>l\<close>
-      apply (subst append_take_drop_id[symmetric, of _ \<open>get_learned_wl S\<close>])
-      unfolding mset_append all_lits_of_mm_union
-      apply (cases S)
-      by (auto simp:  mset_take_mset_drop_mset' literals_are_in_\<L>\<^sub>i\<^sub>n_mm_def clauses_def
-           drop_Suc all_lits_of_mm_union is_\<L>\<^sub>a\<^sub>l\<^sub>l_def)
-    then show ?thesis
-      unfolding literals_are_in_\<L>\<^sub>i\<^sub>n_mm_def by blast
-  qed
-  have pre: \<open>?pre' x\<close> if \<open>?pre x\<close> for x
-    unfolding comp_PRE_def
-    apply (cases x)
-    apply (clarify)
-    apply (intro conjI impI allI)
-    subgoal for L C w i f M N U D NE UE Q W
-      using that find_unwatched_get_clause_neq_L[of f \<open>(M, N, U, D, NE, UE, Q, W)\<close> L w]
-      by (auto simp add: watched_by_app_def)
-    subgoal for L C w i f M N U D NE UE Q W y
-      apply (subgoal_tac \<open>literals_are_in_\<L>\<^sub>i\<^sub>n_mm (mset `# mset (tl N))\<close>)
-      subgoal
-        using literals_are_in_\<L>\<^sub>i\<^sub>n_mm_in_\<L>\<^sub>a\<^sub>l\<^sub>l[of \<open>tl N\<close> \<open>(W L ! w - 1)\<close> f]
-        using that unfolding comp_PRE_def twl_st_heur_def map_fun_rel_def
-          unit_prop_body_wl_D_find_unwatched_inv_def
-          unit_prop_body_wl_find_unwatched_inv_def unit_prop_body_wl_D_inv_def
-          unit_prop_body_wl_inv_def
-          unit_propagation_inner_loop_body_l_inv_def
-        by (auto dest: simp: nth_tl)[]
-      subgoal
-        using that by auto
-      done
-    done
-  have im: \<open>?im' = ?im\<close>
-    unfolding prod_hrp_comp hrp_comp_dest hrp_comp_keep twl_st_assn_def[symmetric]
-    by (auto simp: hrp_comp_def hr_comp_def)
-  have f: \<open>?f' = ?f\<close>
-    unfolding prod_hrp_comp hrp_comp_dest hrp_comp_keep twl_st_assn_def
-    by (auto simp: hrp_comp_def hr_comp_def)
-  show ?thesis
-    apply (rule hfref_weaken_pre[OF ])
-     defer
-    using H unfolding im f PR_CONST_def apply assumption
-    using pre ..
-qed
-
-
 sepref_thm propagate_lit_wl_code
   is \<open>uncurry3 (RETURN oooo (PR_CONST propagate_lit_wl_heur))\<close>
   :: \<open>[propagate_lit_wl_heur_pre]\<^sub>a
@@ -421,44 +164,6 @@ prepare_code_thms (in -) propagate_lit_wl_code_def
 lemmas propagate_lit_wl_code[sepref_fr_rules] =
   propagate_lit_wl_code.refine[OF isasat_input_bounded_nempty_axioms, unfolded PR_CONST_def]
 
-lemma propagate_lit_wl_code_propagate_lit_wl[sepref_fr_rules]:
-  \<open>(uncurry3 propagate_lit_wl_code, uncurry3 (RETURN oooo propagate_lit_wl)) \<in>
-    [\<lambda>(((L, C), i), S). undefined_lit (get_trail_wl S) L \<and> L \<in> snd ` D\<^sub>0 \<and>
-          get_conflict_wl S = None \<and> 1 - i < length (get_clauses_wl S ! C) \<and> i \<le> 1 \<and>
-          C < length (get_clauses_wl S)]\<^sub>a
-     unat_lit_assn\<^sup>k *\<^sub>a nat_assn\<^sup>k *\<^sub>a nat_assn\<^sup>k *\<^sub>a twl_st_assn\<^sup>d \<rightarrow> twl_st_assn\<close>
-    (is \<open>?fun \<in> [?pre]\<^sub>a ?im \<rightarrow> ?f\<close>)
-proof -
-  have H: \<open>?fun \<in>
-     [comp_PRE (Id \<times>\<^sub>f nat_rel \<times>\<^sub>f nat_rel \<times>\<^sub>f twl_st_heur)
-       (\<lambda>(((L, C), i), S). undefined_lit (get_trail_wl S) L \<and> get_conflict_wl S = None)
-       (\<lambda>_ (((L, C), i), S). undefined_lit (get_trail_wl_heur S) L \<and> L \<in> snd ` D\<^sub>0 \<and>
-          1 - i < length (get_clauses_wl_heur S ! C) \<and> i \<le> 1 \<and> C < length (get_clauses_wl_heur S))
-       (\<lambda>_. True)]\<^sub>a
-     hrp_comp (unat_lit_assn\<^sup>k *\<^sub>a nat_assn\<^sup>k *\<^sub>a nat_assn\<^sup>k *\<^sub>a twl_st_heur_assn\<^sup>d)
-                      (Id \<times>\<^sub>f nat_rel \<times>\<^sub>f nat_rel \<times>\<^sub>f twl_st_heur) \<rightarrow>
-     hr_comp twl_st_heur_assn twl_st_heur\<close>
-    (is \<open>_ \<in> [?pre']\<^sub>a ?im' \<rightarrow> ?f'\<close>)
-    using hfref_compI_PRE_aux[OF propagate_lit_wl_code[unfolded PR_CONST_def]
-       propagate_lit_wl_heur_propagate_lit_wl]
-    unfolding propagate_lit_wl_heur_pre_def
-    .
-  have pre: \<open>?pre' x\<close> if \<open>?pre x\<close> for x
-    using that unfolding comp_PRE_def twl_st_heur_def
-    by (auto simp: image_image)
-  have im: \<open>?im' = ?im\<close>
-    unfolding prod_hrp_comp hrp_comp_dest hrp_comp_keep twl_st_assn_def[symmetric]
-    by (auto simp: hrp_comp_def hr_comp_def)
-  have f: \<open>?f' = ?f\<close>
-    unfolding prod_hrp_comp hrp_comp_dest hrp_comp_keep twl_st_assn_def
-    by (auto simp: hrp_comp_def hr_comp_def)
-  show ?thesis
-    apply (rule hfref_weaken_pre[OF ])
-     defer
-    using H unfolding im f PR_CONST_def apply assumption
-    using pre ..
-qed
-
 end
 
 text \<open>Find a less hack-like solution\<close>
@@ -470,70 +175,35 @@ begin
 context
 begin
 
-lemma unit_propagation_inner_loop_body_wl_D_helper:
-  \<open>unit_prop_body_wl_D_inv b ba a \<Longrightarrow> literals_are_in_\<L>\<^sub>i\<^sub>n_trail (get_trail_wl b)\<close>
-  unfolding unit_prop_body_wl_D_inv_def unit_prop_body_wl_inv_def
-  by (rule literals_are_\<L>\<^sub>i\<^sub>n_literals_are_in_\<L>\<^sub>i\<^sub>n_trail[of _ \<open>Some (a, ba)\<close>])
-    auto
-
-sepref_thm unit_propagation_inner_loop_body_wl_D
-  is \<open>uncurry2 ((PR_CONST unit_propagation_inner_loop_body_wl_D) :: nat literal \<Rightarrow> nat \<Rightarrow>
-           nat twl_st_wl \<Rightarrow> (nat \<times> nat twl_st_wl) nres)\<close>
-  :: \<open>unat_lit_assn\<^sup>k *\<^sub>a nat_assn\<^sup>k *\<^sub>a twl_st_assn\<^sup>d \<rightarrow>\<^sub>a nat_assn *a twl_st_assn\<close>
-  supply
-    if_splits[split] unit_prop_body_wl_D_invD[intro,dest]
-    watched_by_app_def[symmetric,simp]
-    access_lit_in_clauses_def[simp] unit_prop_body_wl_D_invD'[intro]
-    length_rll_def[simp] find_unwatched_not_tauto[dest]
-    unit_propagation_inner_loop_body_wl_D_helper[intro]
-  supply undefined_lit_polarity_st_iff[iff]
-  unfolding unit_propagation_inner_loop_body_wl_D_def length_rll_def[symmetric] PR_CONST_def
-  unfolding watched_by_app_def[symmetric] access_lit_in_clauses_def[symmetric]
-    find_unwatched_l_find_unwatched_wl_s
-  unfolding nth_rll_def[symmetric]
-  unfolding lms_fold_custom_empty swap_ll_def[symmetric]
-  unfolding delete_index_and_swap_update_def[symmetric] append_update_def[symmetric]
-    find_unwatched_wl_st_heur_def[symmetric] polarity_st_def[symmetric]
-    set_conflict_wl'_alt_def[symmetric] fast_minus_def[symmetric]
-    SET_FALSE_def[symmetric] SET_TRUE_def[symmetric]
-  supply [[goals_limit=1]]
-  by sepref
-
-
 sepref_register find_unwatched_wl_st_heur
 sepref_thm unit_propagation_inner_loop_body_wl_heur
   is \<open>uncurry2 (PR_CONST unit_propagation_inner_loop_body_wl_heur)\<close>
   :: \<open>unat_lit_assn\<^sup>k *\<^sub>a nat_assn\<^sup>k *\<^sub>a twl_st_heur_assn\<^sup>d \<rightarrow>\<^sub>a nat_assn *a twl_st_heur_assn\<close>
   supply
-    if_splits[split] unit_prop_body_wl_D_invD[intro,dest]
-    watched_by_app_def[symmetric,simp]
-    access_lit_in_clauses_def[simp] unit_prop_body_wl_D_invD'[intro]
-    length_rll_def[simp] find_unwatched_not_tauto[dest]
-    unit_propagation_inner_loop_body_wl_D_helper[intro]
+    if_splits[split]
+    length_rll_def[simp]
     watched_by_app_heur_code_refine[sepref_fr_rules]
   supply undefined_lit_polarity_st_iff[iff]
     unit_prop_body_wl_D_find_unwatched_heur_inv_def[simp]
   unfolding unit_propagation_inner_loop_body_wl_heur_def length_rll_def[symmetric] PR_CONST_def
   unfolding nth_rll_def[symmetric]
-  unfolding lms_fold_custom_empty swap_ll_def[symmetric]
-  unfolding delete_index_and_swap_update_def[symmetric] append_update_def[symmetric]
-    set_conflict_wl'_alt_def[symmetric] fast_minus_def[symmetric]
+  unfolding fast_minus_def[symmetric]
     SET_FALSE_def[symmetric] SET_TRUE_def[symmetric]
   supply [[goals_limit=1]]
   by sepref
 
 end
 
-concrete_definition (in -) unit_propagation_inner_loop_body_wl_D_code
-   uses isasat_input_bounded_nempty.unit_propagation_inner_loop_body_wl_D.refine_raw
+concrete_definition (in -) unit_propagation_inner_loop_body_wl_heur_code
+   uses isasat_input_bounded_nempty.unit_propagation_inner_loop_body_wl_heur.refine_raw
    is \<open>(uncurry2 ?f, _) \<in> _\<close>
 
-prepare_code_thms (in -) unit_propagation_inner_loop_body_wl_D_code_def
+prepare_code_thms (in -) unit_propagation_inner_loop_body_wl_heur_code_def
 
 sepref_register unit_propagation_inner_loop_body_wl_D
 
 lemmas unit_propagation_inner_loop_body_wl_D_code_refine[sepref_fr_rules] =
-   unit_propagation_inner_loop_body_wl_D_code.refine[of \<A>\<^sub>i\<^sub>n, OF isasat_input_bounded_nempty_axioms]
+   unit_propagation_inner_loop_body_wl_heur_code.refine[of \<A>\<^sub>i\<^sub>n, OF isasat_input_bounded_nempty_axioms]
 
 
 paragraph \<open>Unit Propagation, Inner Loop\<close>
@@ -542,7 +212,14 @@ definition (in -) length_ll_fs :: \<open>nat twl_st_wl \<Rightarrow> nat literal
   \<open>length_ll_fs = (\<lambda>(_, _, _, _, _, _, _, W) L. length (W L))\<close>
 
 definition (in -) length_ll_fs_heur :: \<open>twl_st_wl_heur \<Rightarrow> nat literal \<Rightarrow> nat\<close> where
+  \<open>length_ll_fs_heur S L = length (watched_by_int S L)\<close>
+
+lemma length_ll_fs_heur_alt_def:
   \<open>length_ll_fs_heur = (\<lambda>(M, N, U, D, Q, W, _) L. length (W ! nat_of_lit L))\<close>
+  unfolding length_ll_fs_heur_def
+  apply (intro ext)
+  apply (case_tac S)
+  by auto
 
 lemma length_ll_fs_heur_length_ll_fs:
     \<open>(uncurry (RETURN oo length_ll_fs_heur), uncurry (RETURN oo length_ll_fs)) \<in>
@@ -558,7 +235,7 @@ sepref_thm length_ll_fs_heur_code
   is \<open>uncurry (RETURN oo length_ll_fs_heur)\<close>
   :: \<open>[\<lambda>(S, L). nat_of_lit L < length (get_watched_wl_heur S)]\<^sub>a
       twl_st_heur_assn\<^sup>k *\<^sub>a unat_lit_assn\<^sup>k \<rightarrow> nat_assn\<close>
-  unfolding length_ll_fs_heur_def get_watched_wl_heur_def twl_st_heur_assn_def
+  unfolding length_ll_fs_heur_alt_def get_watched_wl_heur_def twl_st_heur_assn_def
     length_ll_def[symmetric]
   supply [[goals_limit=1]]
   by sepref
@@ -572,53 +249,27 @@ prepare_code_thms (in -) length_ll_fs_heur_code_def
 lemmas length_ll_fs_heur_code_refine[sepref_fr_rules] =
    length_ll_fs_heur_code.refine[of \<A>\<^sub>i\<^sub>n, OF isasat_input_bounded_nempty_axioms]
 
-lemma length_ll_fs_heur_code_length_ll_fs[sepref_fr_rules]:
-  \<open>(uncurry length_ll_fs_heur_code, uncurry (RETURN oo length_ll_fs)) \<in>
-    [\<lambda>(S, L). L \<in> snd ` D\<^sub>0]\<^sub>a
-     twl_st_assn\<^sup>k *\<^sub>a unat_lit_assn\<^sup>k \<rightarrow> nat_assn\<close>
-    (is \<open>?fun \<in> [?pre]\<^sub>a ?im \<rightarrow> ?f\<close>)
-proof -
-thm hfref_compI_PRE_aux[OF length_ll_fs_heur_code_refine length_ll_fs_heur_length_ll_fs]
-  have H: \<open>?fun \<in> [comp_PRE (twl_st_heur \<times>\<^sub>f Id) (\<lambda>(S, L). L \<in> snd ` D\<^sub>0)
-    (\<lambda>_ (S, L). nat_of_lit L < length (get_watched_wl_heur S))
-    (\<lambda>_. True)]\<^sub>a hrp_comp (twl_st_heur_assn\<^sup>k *\<^sub>a unat_lit_assn\<^sup>k)
-                   (twl_st_heur \<times>\<^sub>f Id) \<rightarrow> hr_comp nat_assn nat_rel\<close>
-    (is \<open>_ \<in> [?pre']\<^sub>a ?im' \<rightarrow> ?f'\<close>)
-    using hfref_compI_PRE_aux[OF length_ll_fs_heur_code_refine length_ll_fs_heur_length_ll_fs]
-    .
-  have pre: \<open>?pre' x\<close> if \<open>?pre x\<close> for x
-    using that unfolding comp_PRE_def twl_st_heur_def
-    by (auto simp: image_image map_fun_rel_def)
-  have im: \<open>?im' = ?im\<close>
-    unfolding prod_hrp_comp hrp_comp_dest hrp_comp_keep twl_st_assn_def[symmetric]
-    by (auto simp: hrp_comp_def hr_comp_def)
-  have f: \<open>?f' = ?f\<close>
-    unfolding prod_hrp_comp hrp_comp_dest hrp_comp_keep twl_st_assn_def
-    by (auto simp: hrp_comp_def hr_comp_def)
-  show ?thesis
-    apply (rule hfref_weaken_pre[OF ])
-     defer
-    using H unfolding im f PR_CONST_def apply assumption
-    using pre ..
-qed
+sepref_register unit_propagation_inner_loop_body_wl_heur
 
-lemma length_ll_fs_alt_def: \<open>length_ll_fs S L = length_ll_f (watched_by S) L\<close>
-  by (cases S) (auto simp: length_ll_fs_def length_ll_f_def)
-
-sepref_register unit_propagation_inner_loop_wl_loop_D
+thm length_ll_fs_heur_def[symmetric]
+lemma unit_propagation_inner_loop_wl_loop_D_heur_cond:
+  \<open>unit_propagation_inner_loop_wl_loop_D_heur_inv a s' \<Longrightarrow>  s' = (a1', a2') \<Longrightarrow>
+       nat_of_lit a < length (get_watched_wl_heur a2')\<close>
+  by (auto simp: unit_propagation_inner_loop_wl_loop_D_heur_inv_def 
+      twl_st_heur_def map_fun_rel_def)
 
 sepref_thm unit_propagation_inner_loop_wl_loop_D
-  is \<open>uncurry ((PR_CONST unit_propagation_inner_loop_wl_loop_D) :: nat literal \<Rightarrow>
-           nat twl_st_wl \<Rightarrow> (nat \<times> nat twl_st_wl) nres)\<close>
-  :: \<open>unat_lit_assn\<^sup>k *\<^sub>a twl_st_assn\<^sup>d \<rightarrow>\<^sub>a nat_assn *a twl_st_assn\<close>
-  unfolding unit_propagation_inner_loop_wl_loop_D_def PR_CONST_def
+  is \<open>uncurry ((PR_CONST unit_propagation_inner_loop_wl_loop_D_heur))\<close>
+  :: \<open>unat_lit_assn\<^sup>k *\<^sub>a twl_st_heur_assn\<^sup>d \<rightarrow>\<^sub>a nat_assn *a twl_st_heur_assn\<close>
+  unfolding unit_propagation_inner_loop_wl_loop_D_heur_def PR_CONST_def
   unfolding watched_by_nth_watched_app watched_app_def[symmetric]
-    length_ll_f_def[symmetric] length_ll_fs_alt_def[symmetric]
+    length_ll_fs_heur_def[symmetric]
   unfolding nth_ll_def[symmetric]
   unfolding swap_ll_def[symmetric]
   unfolding delete_index_and_swap_update_def[symmetric] append_update_def[symmetric]
-    is_None_def[symmetric] get_conflict_wl_is_None length_ll_fs_def[symmetric]
-  supply [[goals_limit=1]]
+    is_None_def[symmetric] get_conflict_wl_is_None_heur_alt_def[symmetric]
+    length_ll_fs_def[symmetric]
+  supply [[goals_limit=1]] unit_propagation_inner_loop_wl_loop_D_heur_cond[simp]
   by sepref
 
 
@@ -631,12 +282,12 @@ prepare_code_thms (in -) unit_propagation_inner_loop_wl_loop_D_code_def
 lemmas unit_propagation_inner_loop_wl_loop_D_code_refine[sepref_fr_rules] =
    unit_propagation_inner_loop_wl_loop_D_code.refine[of \<A>\<^sub>i\<^sub>n, OF isasat_input_bounded_nempty_axioms]
 
-sepref_register unit_propagation_inner_loop_wl_D
+sepref_register unit_propagation_inner_loop_wl_loop_D_heur
 sepref_thm unit_propagation_inner_loop_wl_D
-  is \<open>uncurry (PR_CONST unit_propagation_inner_loop_wl_D)\<close>
-  :: \<open>unat_lit_assn\<^sup>k *\<^sub>a twl_st_assn\<^sup>d \<rightarrow>\<^sub>a twl_st_assn\<close>
+  is \<open>uncurry (PR_CONST unit_propagation_inner_loop_wl_D_heur)\<close>
+  :: \<open>unat_lit_assn\<^sup>k *\<^sub>a twl_st_heur_assn\<^sup>d \<rightarrow>\<^sub>a twl_st_heur_assn\<close>
   supply [[goals_limit=1]]
-  unfolding PR_CONST_def unit_propagation_inner_loop_wl_D_def
+  unfolding PR_CONST_def unit_propagation_inner_loop_wl_D_heur_def
   by sepref
 
 concrete_definition (in -) unit_propagation_inner_loop_wl_D_code
@@ -651,9 +302,9 @@ lemmas unit_propagation_inner_loop_wl_D_code_refine[sepref_fr_rules] =
 
 paragraph \<open>Unit propagation, Outer Loop\<close>
 
-definition (in -) select_and_remove_from_literals_to_update_wl_heur
+definition (in -) select_and_remove_from_literals_to_update_wl_heur'
   :: \<open>twl_st_wl_heur_W_list \<Rightarrow> twl_st_wl_heur_W_list \<times> _\<close> where
-  \<open>select_and_remove_from_literals_to_update_wl_heur =
+  \<open>select_and_remove_from_literals_to_update_wl_heur' =
      (\<lambda>(M, N, U, D, Q, W, other).  ((M, N, U, D, tl Q, W, other), hd Q))\<close>
 
 definition get_literals_to_update_wl where
@@ -662,33 +313,16 @@ definition get_literals_to_update_wl where
 definition get_literals_to_update_wl_heur_W_list where
    \<open>get_literals_to_update_wl_heur_W_list = (\<lambda>(M, N, U, D, Q, W, _). Q)\<close>
 
-definition literals_to_update_wl_empty_heur :: \<open>twl_st_wl_heur_W_list \<Rightarrow> bool\<close>  where
-  \<open>literals_to_update_wl_empty_heur = (\<lambda>(M, N, U, D, Q, W, oth). Q = [])\<close>
-
-lemma
-  select_and_remove_from_literals_to_update_wl_heur_select_and_remove_from_literals_to_update_wl:
-  \<open>(RETURN o select_and_remove_from_literals_to_update_wl_heur,
-    select_and_remove_from_literals_to_update_wl) \<in>
-    [\<lambda>S. \<not>literals_to_update_wl_empty S]\<^sub>f
-      (twl_st_wl_heur_W_list_rel O twl_st_heur) \<rightarrow>
-       \<langle>(twl_st_wl_heur_W_list_rel O twl_st_heur) \<times>\<^sub>r Id\<rangle>nres_rel\<close>
-  unfolding select_and_remove_from_literals_to_update_wl_heur_def
-  select_and_remove_from_literals_to_update_wl_def get_literals_to_update_wl_heur_W_list_def
-  twl_st_wl_heur_W_list_rel_twl_st_rel get_literals_to_update_wl_def
-  literals_to_update_wl_empty_def
-  apply (intro frefI nres_relI)
-  apply (rename_tac x y, case_tac x, case_tac y,
-      case_tac \<open>get_literals_to_update_wl_heur_W_list y\<close>)
-  unfolding get_literals_to_update_wl_def get_literals_to_update_wl_heur_W_list_def
-  by (auto intro!: RETURN_SPEC_refine simp: nempty_list_mset_rel_iff)
+definition literals_to_update_wl_empty_heur' :: \<open>twl_st_wl_heur_W_list \<Rightarrow> bool\<close>  where
+  \<open>literals_to_update_wl_empty_heur' = (\<lambda>(M, N, U, D, Q, W, oth). Q = [])\<close>
 
 sepref_thm select_and_remove_from_literals_to_update_wl_code
-  is \<open>RETURN o select_and_remove_from_literals_to_update_wl_heur\<close>
-  :: \<open>[\<lambda>S. \<not>literals_to_update_wl_empty_heur S]\<^sub>a
+  is \<open>RETURN o select_and_remove_from_literals_to_update_wl_heur'\<close>
+  :: \<open>[\<lambda>S. \<not>literals_to_update_wl_empty_heur' S]\<^sub>a
       twl_st_heur_W_list_assn\<^sup>d \<rightarrow> twl_st_heur_W_list_assn *a unat_lit_assn\<close>
   supply [[goals_limit=1]]
-  unfolding select_and_remove_from_literals_to_update_wl_heur_def twl_st_heur_W_list_assn_def
-    literals_to_update_wl_empty_heur_def
+  unfolding select_and_remove_from_literals_to_update_wl_heur'_def twl_st_heur_W_list_assn_def
+    literals_to_update_wl_empty_heur'_def
   supply [[goals_limit = 1]]
   by sepref
 
@@ -703,38 +337,60 @@ lemmas select_and_remove_from_literals_to_update_wl_code_refine[sepref_fr_rules]
    select_and_remove_from_literals_to_update_wl_code.refine[of \<A>\<^sub>i\<^sub>n,
      OF isasat_input_bounded_nempty_axioms]
 
+definition literals_to_update_wl_empty_heur :: \<open>twl_st_wl_heur \<Rightarrow> bool\<close>  where
+  \<open>literals_to_update_wl_empty_heur S \<longleftrightarrow> literals_to_update_wl_heur S = {#}\<close>
+
+lemma
+  select_and_remove_from_literals_to_update_wl_heur_select_and_remove_from_literals_to_update_wl:
+  \<open>(RETURN o select_and_remove_from_literals_to_update_wl_heur',
+    select_and_remove_from_literals_to_update_wl_heur) \<in>
+    [\<lambda>S. \<not>literals_to_update_wl_empty_heur S]\<^sub>f
+      (twl_st_wl_heur_W_list_rel) \<rightarrow>
+       \<langle>(twl_st_wl_heur_W_list_rel) \<times>\<^sub>r Id\<rangle>nres_rel\<close>
+  unfolding select_and_remove_from_literals_to_update_wl_heur_def
+    get_literals_to_update_wl_heur_W_list_def
+    twl_st_wl_heur_W_list_rel_twl_st_rel get_literals_to_update_wl_def
+    literals_to_update_wl_empty_heur_def literals_to_update_wl_empty_heur_def
+    select_and_remove_from_literals_to_update_wl_heur'_def literals_to_update_wl_empty_heur_def
+  apply (intro frefI nres_relI)
+  apply (rename_tac x y, case_tac x, case_tac y,
+      case_tac \<open>literals_to_update_wl_empty_heur y\<close>)
+  unfolding get_literals_to_update_wl_def get_literals_to_update_wl_heur_W_list_def
+  by (auto intro!: RETURN_SPEC_refine simp: nempty_list_mset_rel_iff
+      twl_st_wl_heur_W_list_rel_def
+      literals_to_update_wl_empty_heur_def nempty_list_mset_rel_iff)
+
 theorem
   select_and_remove_from_literals_to_update_wl_code_select_and_remove_from_literals_to_update_wl
   [sepref_fr_rules]:
   \<open>(select_and_remove_from_literals_to_update_wl_code,
-     select_and_remove_from_literals_to_update_wl)
-    \<in> [\<lambda>S. \<not> literals_to_update_wl_empty S]\<^sub>a twl_st_assn\<^sup>d \<rightarrow> twl_st_assn *a
+     select_and_remove_from_literals_to_update_wl_heur)
+    \<in> [\<lambda>S. \<not> literals_to_update_wl_empty_heur S]\<^sub>a twl_st_heur_assn\<^sup>d \<rightarrow> twl_st_heur_assn *a
           unat_lit_assn\<close>
     (is \<open>?fun \<in> [?pre]\<^sub>a ?im \<rightarrow> ?f\<close>)
 proof -
   have H: \<open>?fun
-    \<in> [comp_PRE (twl_st_wl_heur_W_list_rel O twl_st_heur)
-         (\<lambda>S. \<not> literals_to_update_wl_empty S)
-         (\<lambda>_ S. \<not> literals_to_update_wl_empty_heur S)
-         (\<lambda>_. True)]\<^sub>a
-      hrp_comp (twl_st_heur_W_list_assn\<^sup>d) (twl_st_wl_heur_W_list_rel O twl_st_heur) \<rightarrow>
-      hr_comp (twl_st_heur_W_list_assn *a unat_lit_assn)
-           ((twl_st_wl_heur_W_list_rel O twl_st_heur) \<times>\<^sub>f Id)\<close>
+    \<in> [comp_PRE twl_st_wl_heur_W_list_rel (\<lambda>S. \<not> literals_to_update_wl_empty_heur S)
+     (\<lambda>_ S. \<not> literals_to_update_wl_empty_heur' S)
+     (\<lambda>_. True)]\<^sub>a hrp_comp (twl_st_heur_W_list_assn\<^sup>d)
+                    twl_st_wl_heur_W_list_rel \<rightarrow> hr_comp (twl_st_heur_W_list_assn *a unat_lit_assn)
+                                                  (twl_st_wl_heur_W_list_rel \<times>\<^sub>f nat_lit_lit_rel)\<close>
      (is \<open>_ \<in> [?pre']\<^sub>a ?im' \<rightarrow> ?f'\<close>)
     using hfref_compI_PRE_aux[OF select_and_remove_from_literals_to_update_wl_code_refine
      select_and_remove_from_literals_to_update_wl_heur_select_and_remove_from_literals_to_update_wl]
     .
   have pre: \<open>?pre' x\<close> if \<open>?pre x\<close> for x
+    apply (cases x)
     using that unfolding comp_PRE_def twl_st_heur_def literals_to_update_wl_empty_heur_def
-      literals_to_update_wl_empty_def twl_st_wl_heur_W_list_rel_def
+      literals_to_update_wl_empty_def twl_st_wl_heur_W_list_rel_def literals_to_update_wl_empty_heur'_def
     by (auto simp: image_image map_fun_rel_def Nil_list_mset_rel_iff)
   have im: \<open>?im' = ?im\<close>
     unfolding prod_hrp_comp hrp_comp_dest hrp_comp_keep twl_st_assn_def[symmetric]
-    twl_st_assn_W_list[symmetric]
+    twl_st_heur_assn_W_list[symmetric]
     by (auto simp: hrp_comp_def hr_comp_def)
   have f: \<open>?f' = ?f\<close>
     unfolding prod_hrp_comp hrp_comp_dest hrp_comp_keep twl_st_assn_def
-    twl_st_assn_W_list[symmetric] hr_comp_prod_conv
+    twl_st_heur_assn_W_list[symmetric] hr_comp_prod_conv
     by (auto simp: hrp_comp_def hr_comp_def)
   show ?thesis
     apply (rule hfref_weaken_pre[OF ])
@@ -744,11 +400,11 @@ proof -
 qed
 
 sepref_thm literals_to_update_wl_empty_heur_code
-  is \<open>RETURN o literals_to_update_wl_empty_heur\<close>
+  is \<open>RETURN o literals_to_update_wl_empty_heur'\<close>
   :: \<open>twl_st_heur_W_list_assn\<^sup>k \<rightarrow>\<^sub>a bool_assn\<close>
   supply [[goals_limit=1]]
-  unfolding select_and_remove_from_literals_to_update_wl_heur_def twl_st_heur_W_list_assn_def
-    literals_to_update_wl_empty_heur_def
+  unfolding select_and_remove_from_literals_to_update_wl_heur'_def twl_st_heur_W_list_assn_def
+    literals_to_update_wl_empty_heur'_def
   supply [[goals_limit = 1]]
   by sepref
 
@@ -762,31 +418,36 @@ lemmas literals_to_update_wl_empty_heur_code_refine[sepref_fr_rules] =
    literals_to_update_wl_empty_heur_code.refine[of \<A>\<^sub>i\<^sub>n, OF isasat_input_bounded_nempty_axioms]
 
 lemma literals_to_update_wl_empty_heur_literals_to_update_wl_empty:
-  \<open>(RETURN o literals_to_update_wl_empty_heur, RETURN o literals_to_update_wl_empty) \<in>
-    twl_st_wl_heur_W_list_rel O twl_st_heur \<rightarrow>\<^sub>f \<langle>Id\<rangle>nres_rel\<close>
-  unfolding literals_to_update_wl_empty_heur_def literals_to_update_wl_empty_def
-    twl_st_wl_heur_W_list_rel_twl_st_rel
+  \<open>(RETURN o literals_to_update_wl_empty_heur', RETURN o literals_to_update_wl_empty_heur) \<in>
+    twl_st_wl_heur_W_list_rel \<rightarrow>\<^sub>f \<langle>Id\<rangle>nres_rel\<close>
+  unfolding literals_to_update_wl_empty_heur_def literals_to_update_wl_empty_heur_def
+    twl_st_wl_heur_W_list_rel_twl_st_rel literals_to_update_wl_empty_heur'_def
   apply (intro frefI nres_relI)
   apply (rename_tac x y, case_tac x, case_tac y)
-  by (auto simp: Nil_list_mset_rel_iff empty_list_mset_rel_iff)
+  by (auto simp: Nil_list_mset_rel_iff empty_list_mset_rel_iff
+      twl_st_wl_heur_W_list_rel_def)
 
 lemma literals_to_update_wl_empty_heur_code_literals_to_update_wl_empty[sepref_fr_rules]:
-  \<open>(literals_to_update_wl_empty_heur_code, RETURN \<circ> literals_to_update_wl_empty)
-     \<in> twl_st_assn\<^sup>k \<rightarrow>\<^sub>a bool_assn\<close>
+  \<open>(literals_to_update_wl_empty_heur_code, RETURN \<circ> literals_to_update_wl_empty_heur)
+     \<in> twl_st_heur_assn\<^sup>k \<rightarrow>\<^sub>a bool_assn\<close>
   using literals_to_update_wl_empty_heur_code_refine[FCOMP
       literals_to_update_wl_empty_heur_literals_to_update_wl_empty]
-  unfolding twl_st_assn_W_list[symmetric]
+  unfolding twl_st_heur_assn_W_list[symmetric]
   .
 
-sepref_register unit_propagation_outer_loop_wl_D
+lemma literals_to_update_wl_literals_to_update_wl_empty:
+  \<open>literals_to_update_wl_heur S = {#} \<longleftrightarrow> literals_to_update_wl_empty_heur S\<close>
+  by (cases S) (auto simp: literals_to_update_wl_empty_def literals_to_update_wl_empty_heur_def)
+
+sepref_register unit_propagation_inner_loop_wl_D_heur
+  select_and_remove_from_literals_to_update_wl_heur
 sepref_thm unit_propagation_outer_loop_wl_D
-  is \<open>((PR_CONST unit_propagation_outer_loop_wl_D) :: nat twl_st_wl \<Rightarrow> (nat twl_st_wl) nres)\<close>
-  :: \<open>twl_st_assn\<^sup>d \<rightarrow>\<^sub>a twl_st_assn\<close>
+  is \<open>PR_CONST unit_propagation_outer_loop_wl_D_heur\<close>
+  :: \<open>twl_st_heur_assn\<^sup>d \<rightarrow>\<^sub>a twl_st_heur_assn\<close>
   supply [[goals_limit=1]]
   apply (subst PR_CONST_def)
-  unfolding unit_propagation_outer_loop_wl_D_def
+  unfolding unit_propagation_outer_loop_wl_D_heur_def
     literals_to_update_wl_literals_to_update_wl_empty
-  supply [[goals_limit = 1]]
   by sepref
 
 concrete_definition (in -) unit_propagation_outer_loop_wl_D
